src/locomp-simple.lean
@@ -1,0 +1,101 @@
+import .love08_operational_semantics_demo .love01_definitions_and_statements_demo
+
+
+-- set_option pp.beta true
+-- set_option pp.generalized_field_notation false
+
+namespace LoComp
+
+open LoVe
+
+def vname := string
+
+def val := ℤ
+
+def stack := list ℤ -- TODO: ???val??? how do we make it accept, because +, -, *, / is not defined for val
+
+def state := vname → val
+
+
+inductive instr : Type  -- page 35 
+| LOADI : val → instr
+| LOAD : vname → instr 
+| ADD : instr
+| SUB : instr
+| MUL : instr
+| DIV : instr
+/-
+| STORE : vname → instr
+| JMP : int → instr
+| JMPLESS : int → instr
+| JMPGE : int → instr
+-/
+
+open instr
+
+def execl : instr → state → stack → stack 
+| (LOADI n) _ stk := n :: stk
+| (LOAD x) s stk :=  (s x) :: stk 
+| ADD _ (j :: i :: stk ) := (i + j) :: stk
+| ADD _ nil := nil  -- anything where it cannot compute
+| SUB _ (j :: i :: stk ) := (i - j) :: stk
+| SUB _ nil := nil
+| MUL _ (j :: i :: stk ) := (i * j) :: stk
+| MUL _ nil := nil
+| DIV _ (j :: i :: stk ) := (i / j) :: stk
+| DIV _ nil := nil
+
+
+
+
+def exec : list instr → state → stack → stack
+| list.nil _ stk := stk
+| (i :: is) s stk := exec is s (execl i s stk)
+
+
+open LoVe.aexp
+
+def comp : aexp → list instr
+| (num n) := [LOADI n]
+| (var x) := [LOAD x]
+| (aexp.add a b) := comp a ++ comp b ++ [ADD] 
+| (aexp.sub a b) := comp a ++ comp b ++ [SUB] 
+| (aexp.mul a b) := comp a ++ comp b ++ [MUL] 
+| (aexp.div a b) := comp a ++ comp b ++ [DIV] 
+
+
+
+
+lemma exec_comp_eq_eval {x : aexp}  {s stk} :
+  exec (comp x) s stk = (eval s x) :: stk :=
+begin
+  induction' x,
+  case LoVe.aexp.num {
+    simp [comp, exec],
+    refl,
+  },
+  case LoVe.aexp.var {
+    simp [comp, exec],
+    refl,
+  },
+  case LoVe.aexp.add {
+    simp [comp, exec],
+    simp [eval],
+    -- simp [comp, exec, ih_x, ih_x_1, eval, add_comm, add_assoc],
+    sorry 
+  },
+  case LoVe.aexp.sub {
+    simp [comp, exec],
+    sorry
+  },
+  case LoVe.aexp.mul {
+    simp [comp, exec],
+    sorry,
+  },
+  case LoVe.aexp.div {
+    simp [comp, exec, ih_x, ih_x_1, eval],
+    sorry,
+  },
+end
+
+end LoComp
